dimsum/itree/small_itree.v
@@ -1,6 +1,6 @@
 From Paco Require Import paco.
 From ITree.Eq Require Import Paco2.
-From dimsum.core.itree Require Export upstream.
+From dimsum.core.itree Require Export upstream events.
 From stdpp Require Import prelude.
 From dimsum.core Require Import base universes.
 
@@ -11,14 +11,14 @@ Local Set Primitive Projections.
 
 Section itree.
 
-  Context {E : TypeBelowState -> TypeState} {R : TypeState}.
+  Context {E : Type -> Type} {R : TypeState} `{!ShrinkEvents E}.
 
   (** The type [itree] is defined as the final coalgebra ("greatest
       fixed point") of the functor [itreeF]. *)
   Variant itreeF (itree : TypeState) :=
   | RetF (r : R)
   | TauF (t : itree)
-  | VisF {X : TypeBelowState} (e : E X) (k : X -> itree)
+  | VisF {X : TypeBelowState} (e : small_events E X) (k : X -> itree)
   .
 
   CoInductive itree : TypeState := go
@@ -26,25 +26,27 @@ Section itree.
 
 End itree.
 
-Arguments itreeF _ _ _ : clear implicits.
-Arguments itree _ _ : clear implicits.
+Arguments itreeF _ _ {_} _.
+Arguments itree _ _ {_}.
 
-Definition from_itree {E : TypeBelowState -> TypeState} {R : TypeState}
+
+Definition from_itree {E : Type -> Type} {R : Type} `{!ShrinkEvents E}
   : ITreeDefinition.itree E R -> itree E R :=
   cofix _from_itree (u : ITreeDefinition.itree E R) : itree E R :=
     match observe u with
     | ITreeDefinition.RetF r => go (RetF r)
     | ITreeDefinition.TauF t => go (TauF (_from_itree t))
-    | ITreeDefinition.VisF e h => go (VisF e (fun x => _from_itree (h x)))
+    | ITreeDefinition.VisF e h => go (VisF (small_events_to_event _ e)
+                                        (fun x => _from_itree (h (small_events_to_back _ e x))))
     end.
 
-Definition to_itree {E : TypeBelowState -> TypeState} {R : TypeState}
+Definition to_itree {E : Type -> Type} {R : TypeState} `{!ShrinkEvents E}
   : itree E R → ITreeDefinition.itree E R :=
   cofix _to_itree (u : itree E R) : ITreeDefinition.itree E R :=
     match _observe u with
     | RetF r => (Ret r)
     | TauF t => (Tau (_to_itree t))
-    | VisF e h => (Vis e (fun x => _to_itree (h x)))
+    | VisF e h => (Vis (small_events_from_event _ e) (fun x => _to_itree (h x)))
     end.
 
 Section from_itree.
@@ -52,10 +54,11 @@ Section from_itree.
     match observe i with
     | ITreeDefinition.RetF r => go (RetF r)
     | ITreeDefinition.TauF t => go (TauF (from_itree t))
-    | ITreeDefinition.VisF e h => go (VisF e (fun x => from_itree (h x)))
+    | ITreeDefinition.VisF e h => go (VisF (small_events_to_event _ e)
+                                        (fun x => from_itree (h (small_events_to_back _ e x))))
     end.
 
-  Lemma unfold_from_itree_ {E R} (t : ITreeDefinition.itree E R)
+  Lemma unfold_from_itree_ {E R} (t : ITreeDefinition.itree E R) `{!ShrinkEvents E}
     : eq (_observe (from_itree t)) (_observe (from_itree_ t)).
   Proof. constructor; reflexivity. Qed.
 End from_itree.
@@ -65,16 +68,16 @@ Section to_itree.
     match _observe i with
     | RetF r => (Ret r)
     | TauF t => (Tau (to_itree t))
-    | VisF e h => (Vis e (fun x => to_itree (h x)))
+    | VisF e h => (Vis (small_events_from_event _ e) (fun x => to_itree (h x)))
     end.
 
-  Lemma unfold_to_itree_ {E R} (t : itree E R)
+  Lemma unfold_to_itree_ {E R} `{!ShrinkEvents E} (t : itree E R)
     : observing eq (to_itree t) (to_itree_ t).
   Proof. constructor; reflexivity. Qed.
 End to_itree.
 
 
-Lemma from_to_itree E R (i : ITreeDefinition.itree E R) :
+Lemma from_to_itree E R `{!ShrinkEvents E} (i : ITreeDefinition.itree E R) :
   to_itree (from_itree i) ≅ i.
 Proof.
   revert i. ginit. pcofix IH => i.
@@ -83,33 +86,33 @@ Proof.
   destruct (observe i); simpl.
   - gstep. by constructor.
   - gstep. constructor. eauto with paco.
-  - gstep. constructor => ? /=. eauto with paco.
+  - gstep. rewrite -(small_events_eq (λ T e k, Vis e k) _ k). constructor => ? /=. eauto with paco.
 Qed.
 
-Global Instance SmallITree_equiv {E R} : Equiv (itree E R) :=
+Global Instance SmallITree_equiv {E R} `{!ShrinkEvents E} : Equiv (itree E R) :=
   λ t1 t2, SmallITree.to_itree t1 ≅ SmallITree.to_itree t2.
 
-Lemma equiv_from_itree E R (x y : ITreeDefinition.itree E R) :
+Lemma equiv_from_itree E R `{!ShrinkEvents E} (x y : ITreeDefinition.itree E R) :
   from_itree x ≡ from_itree y ↔ x ≅ y.
 Proof.
   unfold equiv, SmallITree_equiv. by rewrite !from_to_itree.
 Qed.
 
-Lemma eqit_to_itree E R (x y : itree E R) :
+Lemma eqit_to_itree E R `{!ShrinkEvents E} (x y : itree E R) :
   to_itree x ≅ to_itree y ↔ x ≡ y.
 Proof. done. Qed.
 
-Global Instance SmallITree_equiv_proper E R :
-  Proper ((eq_itree eq) ==> (≡)) (@SmallITree.from_itree E R).
+Global Instance SmallITree_equiv_proper E R `{!ShrinkEvents E} :
+  Proper ((eq_itree eq) ==> (≡)) (@SmallITree.from_itree E R _).
 Proof. intros ?? Heq. by apply equiv_from_itree. Qed.
 
-Global Instance SmallITree_to_itree_proper E R :
-  Proper ((≡) ==> (eq_itree eq)) (@SmallITree.to_itree E R).
+Global Instance SmallITree_to_itree_proper E R `{!ShrinkEvents E} :
+  Proper ((≡) ==> (eq_itree eq)) (@SmallITree.to_itree E R _).
 Proof. intros ?? Heq. by apply eqit_to_itree. Qed.
 
-Global Instance SmallITree_equiv_rewrite {E R} : RewriteRelation (≡@{itree E R}) := { }.
+Global Instance SmallITree_equiv_rewrite {E R} `{!ShrinkEvents E} : RewriteRelation (≡@{itree E R}) := { }.
 
-Global Instance SmallITree_equiv_equiv {E R} : Equivalence (≡@{itree E R}).
+Global Instance SmallITree_equiv_equiv {E R} `{!ShrinkEvents E} : Equivalence (≡@{itree E R}).
 Proof.
   unfold equiv, SmallITree_equiv.
   constructor.
@@ -118,33 +121,33 @@ Proof.
   - intros ??? ->. done.
 Qed.
 
-Global Instance SmallITree_supseteq {E R} : SqSupsetEq (itree E R) :=
+Global Instance SmallITree_supseteq {E R} `{!ShrinkEvents E} : SqSupsetEq (itree E R) :=
   λ t1 t2, SmallITree.to_itree t1 ≳ SmallITree.to_itree t2.
 
-Lemma supseteq_from_itree E R (x y : ITreeDefinition.itree E R) :
+Lemma supseteq_from_itree E R `{!ShrinkEvents E} (x y : ITreeDefinition.itree E R) :
   from_itree x ⊒ from_itree y ↔ x ≳ y.
 Proof.
   unfold sqsupseteq, SmallITree_supseteq. by rewrite !from_to_itree.
 Qed.
 
-Lemma euttge_to_itree E R (x y : itree E R) :
+Lemma euttge_to_itree E R `{!ShrinkEvents E} (x y : itree E R) :
   to_itree x ≳ to_itree y ↔ x ⊒ y.
 Proof. done. Qed.
 
-Global Instance SmallITree_supseteq_proper_equiv E R :
+Global Instance SmallITree_supseteq_proper_equiv E R `{!ShrinkEvents E} :
   Proper ((≡) ==> (≡) ==> iff) (⊒@{SmallITree.itree E R}).
 Proof.
   unfold equiv, SmallITree_equiv, sqsupseteq, SmallITree_supseteq.
   intros ?? Heq1 ?? Heq2. by rewrite Heq1 Heq2.
 Qed.
-Global Instance SmallITree_supseteq_proper E R :
-  Proper ((euttge eq) ==> (⊒)) (@SmallITree.from_itree E R).
+Global Instance SmallITree_supseteq_proper E R `{!ShrinkEvents E} :
+  Proper ((euttge eq) ==> (⊒)) (@SmallITree.from_itree E R _).
 Proof. intros ?? Heq. by apply supseteq_from_itree. Qed.
-Global Instance SmallITree_supseteq_proper_flip E R :
-  Proper (flip (euttge eq) ==> flip (⊒)) (@SmallITree.from_itree E R).
+Global Instance SmallITree_supseteq_proper_flip E R `{!ShrinkEvents E} :
+  Proper (flip (euttge eq) ==> flip (⊒)) (@SmallITree.from_itree E R _).
 Proof. intros ?? Heq. by apply supseteq_from_itree. Qed.
 
-Global Instance SmallITree_supseteq_preorder {E R} : PreOrder (⊒@{itree E R}).
+Global Instance SmallITree_supseteq_preorder {E R} `{!ShrinkEvents E} : PreOrder (⊒@{itree E R}).
 Proof.
   unfold sqsupseteq, SmallITree_supseteq.
   constructor.
@@ -156,7 +159,7 @@ End SmallITree.
 Notation "↓ᵢ" := SmallITree.from_itree : stdpp_scope.
 Notation "↑ᵢ" := SmallITree.to_itree : stdpp_scope.
 
-From dimsum.core.itree Require Export events.
-
+(* Should be able to solve ShrinkEvents *)
 Check ∀ t : itree (stateE nat +' choiceE +' visibleE nat) unit, SmallITree.from_itree t = SmallITree.from_itree t.
-Fail Check ∀ t : itree (choiceE +' visibleE (itree choiceE nat)) unit, SmallITree.from_itree t = SmallITree.from_itree t.
+(* Should not be able to solve ShrinkEvents *)
+Check ∀ t : itree (choiceE +' visibleE (itree choiceE nat)) unit, SmallITree.from_itree t = SmallITree.from_itree t.
