dimsum/irefines.v
@@ -1,0 +1,117 @@
+From dimsum.core Require Import module trefines.
+From dimsum.core.itree Require Import upstream events.
+Import ITreeStdppNotations.
+
+(** * [irefines] *)
+Inductive ihas_trace {EV S} : itree (moduleE_big EV S) void → S → trace EV → (itree (moduleE_big EV S) void → S → Prop) → Prop :=
+| ITraceTau t t' σ κs Pσ:
+  t ≅ Tau t' →
+  ihas_trace t' σ κs Pσ →
+  ihas_trace t σ κs Pσ
+| ITraceAngelicBig T t t' σ κs Pσ:
+  t ≅ (Vis (inl1 (EAngelic_big T)) t') →
+  (∀ x, ihas_trace (t' x) σ κs Pσ) →
+  ihas_trace t σ κs Pσ
+| ITraceDemonicBig T t t' σ κs Pσ x:
+  t ≅ (Vis (inl1 (EDemonic_big T)) t') →
+  ihas_trace (t' x) σ κs Pσ →
+  ihas_trace t σ κs Pσ
+| ITraceAngelic T t t' σ κs Pσ:
+  t ≅ (Vis (inr1 (inl1 (EAngelic T))) t') →
+  (∀ x, ihas_trace (t' x) σ κs Pσ) →
+  ihas_trace t σ κs Pσ
+| ITraceDemonic T t t' σ κs Pσ x:
+  t ≅ (Vis (inr1 (inl1 (EDemonic T))) t') →
+  ihas_trace (t' x) σ κs Pσ →
+  ihas_trace t σ κs Pσ
+| ITraceVis e t t' σ κs κs' Pσ:
+  t ≅ (Vis (inr1 (inr1 (inl1 (EVisible e)))) t') →
+  tcons e κs' ⊆ κs →
+  ihas_trace (t' ()) σ κs' Pσ →
+  ihas_trace t σ κs Pσ
+| ITraceGetState t t' σ κs Pσ:
+  t ≅ (Vis (inr1 (inr1 (inr1 EGetState))) t') →
+  ihas_trace (t' σ) σ κs Pσ →
+  ihas_trace t σ κs Pσ
+| ITraceSetState t t' σ σ' κs Pσ:
+  t ≅ (Vis (inr1 (inr1 (inr1 (ESetState σ')))) t') →
+  ihas_trace (t' ()) σ' κs Pσ →
+  ihas_trace t σ κs Pσ
+| ITraceAll t T f σ κs Pσ:
+    (∀ x, ihas_trace t σ (f x) Pσ) →
+    tall T f ⊆ κs →
+    ihas_trace t σ κs Pσ
+| ITraceEnd t t' σ (Pσ : _ → _ → Prop) κs:
+  t ≅ t' →
+  Pσ t' σ →
+  tnil ⊆ κs →
+  ihas_trace t σ κs Pσ
+.
+
+(* TODO: Better notation where σ is not in the braces? *)
+Notation " t '~{' σ , κs '}~>ᵢ' P " := (ihas_trace t σ κs P) (at level 40).
+Notation " t '~{' σ , κs '}~>ᵢ' - " := (ihas_trace t σ κs (λ _ _, True)) (at level 40).
+
+Global Instance ihas_trace_proper {EV S} :
+  Proper (eq_itree eq ==> (=) ==> (⊆) ==> (pointwise_relation _ (pointwise_relation S impl)) ==> impl) (@ihas_trace EV S).
+Proof.
+  move => t1 t2 Heq ?? -> κs1 κs2 Hκs Pσ1 Pσ2 HP Ht.
+  elim: Ht t2 κs2 Pσ2 Heq Hκs HP.
+  - move => *. econstructor; [by etrans|naive_solver].
+  - move => *. econstructor; [by etrans|naive_solver].
+  - move => *. econstructor; [by etrans|naive_solver].
+  - move => *. econstructor; [by etrans|naive_solver].
+  - move => *. econstructor; [by etrans|naive_solver].
+  - move => *. econstructor; [by etrans|..]. 1: by etrans; [|done]. naive_solver.
+  - move => *. econstructor; [by etrans|naive_solver].
+  - move => *. econstructor; [by etrans|naive_solver].
+  - move => *. apply: ITraceAll; [|by etrans]. naive_solver.
+  - move => ????????????? HP. apply: ITraceEnd; [ | by apply: HP | by etrans].
+    by etrans.
+Qed.
+
+Global Instance ihas_trace_proper_flip {EV S} :
+  Proper ((eq_itree eq) ==> (=) ==> (flip (⊆)) ==> (=) ==> flip impl) (@ihas_trace EV S).
+Proof. move => ?? Ht ?? -> ?? Hsub ?? -> /=. by rewrite Hsub Ht. Qed.
+
+Lemma ihas_trace_mono {EV S} (t : itree (moduleE_big EV S) void) κs' κs (Pσ2' Pσ2 : _ → _ → Prop)  σ :
+  t ~{ σ, κs' }~>ᵢ Pσ2' →
+  κs' ⊆ κs →
+  (∀ t σ, Pσ2' t σ → Pσ2 t σ) →
+  t ~{ σ, κs }~>ᵢ Pσ2.
+Proof. move => ???. by apply: ihas_trace_proper. Qed.
+
+Record irefines {EV Si Ss} (ti : itree (moduleE_big EV Si) void) (σi : Si)
+  (ts : itree (moduleE_big EV Ss) void) (σs : Ss) : Prop := {
+  iref_subset:
+    ∀ κs, ti ~{ σi, κs }~>ᵢ - →
+          ts ~{ σs, κs }~>ᵢ -
+}.
+
+(** * Relating irefines to trefines *)
+Definition mod_to_itree {EV} (m : mod_trans EV) : itree (moduleE_big EV (m.(m_state))) void:=
+  ITree.forever (
+      σ ← get_state;
+      Pσ' ← demonic_big _;
+      κ ← demonic _;
+      assert (m.(m_step) σ κ Pσ');;
+      (if κ is Some e then visible e else Ret ());;
+      σ' ← angelic_big _;
+      assume (Pσ' σ');;
+      set_state σ')%itree.
+
+Lemma thas_trace_ihas_trace EV (m : mod_trans EV) σ κs :
+  σ ~{m, κs}~>ₜ - ↔ mod_to_itree m ~{σ, κs}~>ᵢ -.
+Proof.
+Admitted.
+
+Lemma irefines_trefines EV (mi ms : module EV) :
+  trefines mi ms ↔ irefines (mod_to_itree mi.(m_trans)) mi.(m_init)
+                            (mod_to_itree ms.(m_trans)) ms.(m_init).
+Proof.
+  split; move => [Hr]; constructor => κs; move: (Hr κs).
+  all: by rewrite !thas_trace_ihas_trace.
+Qed.
+
+(* Import here to check that there are not universe inconsistencies *)
+From dimsum.core.itree Require Import asm rec.
